programming_language_foundations/StlcProp.v
@@ -333,3 +333,425 @@ Module STLCProp.
   Qed.
 
   End STLCProp.
+
+Module STLCArith.
+  Import STLC.
+
+  Inductive ty : Type :=
+  | Arrow : ty -> ty -> ty
+  | Nat : ty.
+
+  Inductive tm : Type :=
+  | var : string -> tm
+  | app : tm -> tm -> tm
+  | abs : string -> ty -> tm -> tm
+  | const : nat -> tm
+  | scc : tm -> tm
+  | prd : tm -> tm
+  | mlt : tm -> tm -> tm
+  | test0 : tm -> tm -> tm -> tm.
+
+  Reserved Notation "'[' x ':=' s ']' t" (at level 20).
+
+  Fixpoint subst (x : string) (s : tm) (t : tm) : tm :=
+    match t with
+    | var x' =>
+      if eqb_string x x' then s else t
+    | abs x' T t1 =>
+      abs x' T (if eqb_string x x' then t1 else ([x:=s] t1))
+    | app t1 t2 =>
+      app ([x:=s] t1) ([x:=s] t2)
+    | const n => const n
+    | scc t' => scc ([x:=s] t')
+    | prd t' => prd ([x:=s] t')
+    | mlt t1 t2 => mlt ([x:=s] t1) ([x:=s] t2)
+    | test0 t1 t2 t3 =>
+      test0 ([x:=s] t1) ([x:=s] t2) ([x:=s] t3)
+    end
+  where "'[' x ':=' s ']' t" := (subst x s t).
+
+  Inductive value : tm -> Prop :=
+  | v_abs : forall x T t, value (abs x T t)
+  | v_const : forall n, value (const n).
+
+  Hint Constructors value : db.
+
+  Reserved Notation "t1 '-->' t2" (at level 40).
+
+  Inductive step : tm -> tm -> Prop :=
+  | ST_AppAbs : forall x T t12 v2,
+      value v2 ->
+      (app (abs x T t12) v2) --> [x:=v2]t12
+  | ST_App1 : forall t1 t1' t2,
+      t1 --> t1' ->
+      app t1 t2 --> app t1' t2
+  | ST_App2 : forall v1 t2 t2',
+      value v1 ->
+      t2 --> t2' ->
+      app v1 t2 --> app v1 t2'
+  | ST_Scc1 : forall t1 t1',
+      t1 --> t1' ->
+      scc t1 --> scc t1'
+  | ST_Scc2 : forall n,
+      scc (const n) --> const (n+1)
+  | ST_Prd1 : forall t1 t1',
+      t1 --> t1' ->
+      prd t1 --> prd t1'
+  | ST_Prd2 : forall n,
+      prd (const n) --> const (n - 1)
+  | ST_Mlt1 : forall t1 t1' t2,
+      t1 --> t1' ->
+      mlt t1 t2 --> mlt t1' t2
+  | ST_Mlt2 : forall n1 t2 t2',
+      value (const n1) ->
+      t2 --> t2' ->
+      mlt (const n1) t2 --> mlt (const n1) t2'
+  | ST_Mlt3 : forall n1 n2,
+      value (const n1) ->
+      value (const n2) ->
+      mlt (const n1) (const n2) --> const (n1 * n2)
+  | ST_TestZero : forall t1 t2,
+      (test0 (const 0) t1 t2) --> t2
+  | ST_TestNonZero : forall v1 t1 t2,
+      v1 > 0 ->
+      (test0 (const v1) t1 t2) --> t1
+  | ST_Test : forall t1 t1' t2 t3,
+      t1 --> t1' ->
+      (test0 t1 t2 t3) --> (test0 t1' t2 t3)
+  where "t1 '-->' t2" := (step t1 t2).
+
+  Hint Constructors step : db.
+
+  Definition context := partial_map ty.
+  
+  Reserved Notation "Gamma '|-' t '?' T" (at level 40).
+  Inductive has_type : context -> tm -> ty -> Prop :=
+  | T_Var : forall Gamma x T,
+      Gamma x = Some T ->
+      Gamma |- var x ? T
+  | T_Abs : forall Gamma x T11 T12 t12,
+      (x |-> T11; Gamma) |- t12 ? T12 ->
+      Gamma |- abs x T11 t12 ? Arrow T11 T12
+  | T_App : forall T11 T12 Gamma t1 t2,
+      Gamma |- t1 ? Arrow T11 T12 ->
+      Gamma |- t2 ? T11 ->
+      Gamma |- app t1 t2 ? T12
+  | T_Const : forall Gamma n,
+      Gamma |- const n ? Nat
+  | T_Scc : forall Gamma t,
+      Gamma |- t ? Nat ->
+      Gamma |- scc t ? Nat
+  | T_Prd : forall Gamma t,
+      Gamma |- t ? Nat ->
+      Gamma |- prd t ? Nat
+  | T_Mlt : forall Gamma t1 t2,
+      Gamma |- t1 ? Nat ->
+      Gamma |- t2 ? Nat ->
+      Gamma |- mlt t1 t2 ? Nat
+  | T_Test0 : forall t1 t2 t3 T Gamma,
+      Gamma |- t1 ? Nat ->
+      Gamma |- t2 ? T ->
+      Gamma |- t3 ? T ->
+      Gamma |- test0 t1 t2 t3 ? T
+  where "Gamma '|-' t '?' T" := (has_type Gamma t T).
+
+  Hint Constructors has_type : db.
+
+  Inductive appears_free_in : string -> tm -> Prop :=
+  | afi_var : forall x,
+      appears_free_in x (var x)
+  | afi_app1 : forall x t1 t2,
+      appears_free_in x t1 ->
+      appears_free_in x (app t1 t2)
+  | afi_app2 : forall x t1 t2,
+      appears_free_in x t2 ->
+      appears_free_in x (app t1 t2)
+  | afi_abs : forall x y T11 t12,
+      y <> x ->
+      appears_free_in x t12 ->
+      appears_free_in x (abs y T11 t12)
+  | afi_scc : forall x t1,
+      appears_free_in x t1 ->
+      appears_free_in x (scc t1)
+  | afi_prd : forall x t1,
+      appears_free_in x t1 ->
+      appears_free_in x (prd t1)
+  | afi_mlt1 : forall x t1 t2,
+      appears_free_in x t1 ->
+      appears_free_in x (mlt t1 t2)
+  | afi_mlt2 : forall x t1 t2,
+      appears_free_in x t2 ->
+      appears_free_in x (mlt t1 t2)
+  | afi_test1 : forall x t1 t2 t3 ,
+      appears_free_in x t1 ->
+      appears_free_in x (test0 t1 t2 t3)
+  | afi_test2 : forall x t1 t2 t3,
+      appears_free_in x t2 ->
+      appears_free_in x (test0 t1 t2 t3)
+  | afi_test3 : forall x t1 t2 t3,
+      appears_free_in x t3 ->
+      appears_free_in x (test0 t1 t2 t3).
+  
+  Hint Constructors appears_free_in : db.
+
+  Lemma context_invariance : forall Gamma Gamma' t T,
+      Gamma |- t ? T ->
+      (forall x, appears_free_in x t -> Gamma x = Gamma' x) ->
+      Gamma' |- t ? T.
+  Proof.
+    intros Gamma Gamma' t T H1 H2.
+    generalize dependent Gamma'.
+    induction H1; intros Gamma' H2.
+    - apply T_Var. rewrite <- H. symmetry.
+      eapply H2. apply afi_var.
+    - apply T_Abs. apply IHhas_type.
+      intros x1 Hafi. destruct (string_dec x0 x1).
+      + rewrite e. rewrite update_eq. rewrite update_eq.
+        reflexivity.
+      + rewrite update_neq.
+        * rewrite update_neq.
+          { apply H2. apply afi_abs. apply n. apply Hafi. }
+          { apply n. }
+        * apply n.
+    - eapply T_App.
+      + apply IHhas_type1. intros x0 H3.
+        apply H2. apply afi_app1. apply H3.
+      + apply IHhas_type2. intros x0 H3.
+        apply H2. apply afi_app2. apply H3.
+    - apply T_Const.
+    - apply T_Scc. apply IHhas_type. intros x0 H3.
+      apply H2. apply afi_scc. apply H3.
+    - apply T_Prd. apply IHhas_type. intros x0 H3.
+      apply H2. apply afi_prd. apply H3.
+    - apply T_Mlt.
+      + apply IHhas_type1. intros x0 H3.
+        apply H2. apply afi_mlt1. apply H3.
+      + apply IHhas_type2. intros x0 H3.
+        apply H2. apply afi_mlt2. apply H3.
+    - apply T_Test0.
+      + apply IHhas_type1. intros x0 H3.
+        apply H2. apply afi_test1. apply H3.
+      + apply IHhas_type2. intros x0 H3.
+        apply H2. apply afi_test2. apply H3.
+      + apply IHhas_type3. intros x0 H3.
+        apply H2. apply afi_test3. apply H3.
+  Qed.
+
+  Lemma free_in_context : forall x t T Gamma,
+      appears_free_in x t ->
+      Gamma |- t ? T ->
+      exists T', Gamma x = Some T'.
+  Proof.
+    intros x t T Gamma Hafi.
+    generalize dependent Gamma. generalize dependent T.
+    induction Hafi.
+    - intros T Gamma H. inversion H; subst. eapply ex_intro. apply H2.
+    - intros T Gamma H. inversion H; subst.
+      eapply IHHafi. apply H3.
+    - intros T Gamma H. inversion H; subst. eapply IHHafi. apply H5.
+    - intros T Gamma H1. inversion H1; subst.
+      apply (IHHafi T12 (y0 |-> T11; Gamma)) in H6.
+      destruct H6. rewrite update_neq in H0.
+      + eexists. apply H0.
+      + apply H.
+    - intros T Gamma H. inversion H; subst.
+      eapply IHHafi. apply H2.
+    - intros T Gamma H. inversion H; subst.
+      eapply IHHafi. apply H2.
+    - intros T Gamma H. inversion H; subst.
+      eapply IHHafi. apply H3.
+    - intros T Gamma H. inversion H; subst.
+      eapply IHHafi. apply H5.
+    - intros T Gamma H. inversion H; subst.
+      eapply IHHafi. apply H4.
+    - intros T Gamma H. inversion H; subst.
+      eapply IHHafi. apply H6.
+    - intros T Gamma H. inversion H; subst.
+      eapply IHHafi. apply H7.
+  Qed.
+  
+  Definition closed (t : tm) :=
+    forall x, ~ appears_free_in x t.
+  
+  Corollary typable_empty__closed : forall t T,
+      empty |- t ? T ->
+      closed t.
+  Proof.
+    unfold closed. intros t T H x0 H1.
+    apply (free_in_context x0 t T empty H1) in H.
+    inversion H. inversion H0.
+  Qed.
+  
+  Lemma substitution_preserves_typing : forall Gamma x U t v T,
+      (x |-> U; Gamma) |- t ? T ->
+      empty |- v ? U ->
+      Gamma |- [x:=v]t ? T.
+  Proof with eauto.
+    intros Gamma x U t v T Ht Ht'.
+    generalize dependent Gamma. generalize dependent T.
+    induction t; intros T Gamma H; inversion H; subst; simpl...
+    - rename s into y. destruct (eqb_stringP x y) as [Hxy|Hxy].
+      + subst. rewrite update_eq in H2. inversion H2; subst.
+        eapply context_invariance. eassumption.
+        apply typable_empty__closed in Ht'. unfold closed in Ht'.
+        intros. apply (Ht' x0) in H0. inversion H0.
+      + apply T_Var. rewrite update_neq in H2...
+    - eapply T_App.
+      + apply IHt1. apply H3.
+      + apply IHt2. apply H5.
+    - rename s into y. rename t into T. apply T_Abs.
+      destruct (eqb_stringP x y) as [Hxy | Hxy].
+      + subst. rewrite update_shadow in H5. apply H5.
+      + apply IHt. eapply context_invariance...
+        intros z Hafi.
+        destruct (string_dec y z).
+        * subst. rewrite update_eq.
+          destruct (string_dec x z).
+          { subst. rewrite update_eq. exfalso.
+            apply Hxy. reflexivity. }
+          { rewrite update_neq. rewrite update_eq.
+            reflexivity. apply n. 
+          }
+        * rewrite update_neq. destruct (string_dec x z).
+          { subst. rewrite update_eq. rewrite update_eq. reflexivity. }
+          { rewrite update_neq. rewrite update_neq. rewrite update_neq.
+            reflexivity. apply n. apply n0. apply n0.
+          }
+          { apply n. }
+    - apply T_Const.
+    - apply T_Scc. apply IHt. apply H2.
+    - apply T_Prd. apply IHt. apply H2.
+    - apply T_Mlt.
+      + apply IHt1. apply H3.
+      + apply IHt2. apply H5.
+    - apply T_Test0.
+      + apply IHt1. apply H4.
+      + apply IHt2. apply H6.
+      + apply IHt3. apply H7.
+  Qed.
+  
+  Theorem preservation : forall t t' T,
+      empty |- t ? T ->
+      t --> t' ->
+      empty |- t' ? T.
+  Proof with eauto.
+    remember (@empty ty) as Gamma.
+    intros t t' T HT. generalize dependent t'.
+    induction HT; intros t' HE.
+    - subst Gamma. subst. solve [inversion HE; subst; auto].
+    - subst Gamma. subst. solve [inversion HE; subst; auto].
+    - subst. inversion HE; subst...
+      + apply substitution_preserves_typing with T11...
+        inversion HT1...
+      + eapply T_App.
+        * apply IHHT1. reflexivity. apply H2.
+        * apply HT2.
+      + eapply T_App.
+        * apply HT1.
+        * apply IHHT2. reflexivity. apply H3.
+    - inversion HE.
+    - inversion HE; subst.
+      + apply T_Scc. apply IHHT.
+        * reflexivity.
+        * apply H0.
+      + apply T_Const. 
+    - inversion HE; subst.
+      + apply T_Prd. apply IHHT.
+        * reflexivity. 
+        * apply H0.
+      + apply T_Const.
+    - inversion HE; subst.
+      + apply T_Mlt.
+        * apply IHHT1.
+          reflexivity.
+          apply H2.
+        * apply HT2.
+      + apply T_Mlt.
+        * apply HT1.
+        * apply IHHT2.
+          reflexivity.
+          apply H3.
+      + apply T_Const.
+    - inversion HE; subst.
+      + apply HT3.
+      + apply HT2.
+      + apply T_Test0.
+        * apply IHHT1. reflexivity. apply H3.
+        * apply HT2.
+        * apply HT3.
+  Qed.
+
+  Lemma canonical_forms_fun : forall t T1 T2,
+      empty |- t ? (Arrow T1 T2) ->
+      value t ->
+      exists x u, t = abs x T1 u.
+  Proof.
+    intros t T1 T2 H1 Hv.
+    inversion H1; subst; inversion Hv.
+    eexists. eexists. reflexivity.
+  Qed.
+  
+  Theorem progress : forall t T,
+      empty |- t ? T ->
+      value t \/ exists t', t --> t'.
+  Proof.
+    intros t T H.
+    remember (@empty ty) as Gamma.
+    induction H.
+    - subst. inversion H.
+    - left. apply v_abs.
+    - right. destruct IHhas_type1; subst.
+      + reflexivity. 
+      + destruct IHhas_type2; subst.
+        * reflexivity. 
+        * apply (canonical_forms_fun t1 T11 T12 H) in H1.
+          destruct H1. destruct H1. subst.
+          eexists. apply ST_AppAbs. apply H2.
+        * subst. destruct H2.  eexists. apply ST_App2. apply H1. 
+          apply H2.
+      + subst. destruct H1. eexists. apply ST_App1. apply H1.
+    - subst. left. apply v_const.
+    - subst. destruct IHhas_type.
+      + reflexivity.
+      + right. inversion H0; subst.
+        * inversion H.
+        * eexists. apply ST_Scc2.
+      + right. inversion H0. eexists. apply ST_Scc1. apply H1.
+    - subst. destruct IHhas_type.
+      + reflexivity.
+      + right. inversion H0; subst.
+        * inversion H.
+        * eexists. apply ST_Prd2.
+      + right. inversion H0. eexists. apply ST_Prd1. apply H1.
+    - subst. destruct IHhas_type1.
+      + reflexivity.
+      + destruct IHhas_type2.
+        * reflexivity.
+        * inversion H1; subst.
+          { inversion H. }
+          { inversion H2; subst.
+            { inversion H0. }
+            { right. eexists. apply ST_Mlt3; assumption. }
+          }
+        * right. inversion H1; subst.
+          { inversion H. }
+          { destruct H2. eexists. apply ST_Mlt2. apply H1. apply H2. }
+      + right. destruct H1. eexists. apply ST_Mlt1. apply H1.
+    - subst.
+      assert (Heq1 : value t1 \/ (exists t' : tm, t1 --> t')).
+      { apply IHhas_type1. reflexivity. }
+      assert (Heq2 : value t2 \/ (exists t' : tm, t2 --> t')).
+      { apply IHhas_type2. auto. }
+      assert (Heq3 : value t3 \/ (exists t' : tm, t3 --> t')).
+      { auto. }
+      destruct Heq1.
+      + inversion H2; subst.
+        * inversion H.
+        * destruct n.
+          { right. eexists. apply ST_TestZero. }
+          { right. eexists. apply ST_TestNonZero. apply Gt.gt_Sn_O. }
+      + destruct H2; subst. right.
+        eexists. apply ST_Test. apply H2.
+  Qed.
+
+End STLCArith.
